fixed: accidentally deletes

src/dvspec/dafny/att_spec_proofs/inv.dfy
@@ -125,14 +125,14 @@ module Att_Inv_With_Empty_Initial_Attestation_Slashing_DB
     }
 
     // If the current duty is not none, then the lastest served duty is the current duty.
-    predicate inv5(dvn: DVState)        
+    predicate old_inv5(dvn: DVState)        
     {
         forall pubkey: BLSPubkey | is_honest_node(dvn, pubkey) ::
             && var s := dvn.honest_nodes_states[pubkey];
-            && inv5_body(s)            
+            && old_inv5_body(s)            
     }
 
-    predicate inv5_body(hn_state: DVCNodeState)        
+    predicate old_inv5_body(hn_state: DVCNodeState)        
     {
         hn_state.current_attestation_duty.isPresent()
             ==> ( && hn_state.latest_attestation_duty.isPresent()
@@ -1488,6 +1488,15 @@ module Att_Inv_With_Empty_Initial_Attestation_Slashing_DB
 
     predicate inv3(dvn: DVState)
     {
+        forall n | n in dvn.honest_nodes_states.Keys :: 
+            var nodes := dvn.honest_nodes_states[n];
+            && nodes.construct_signed_attestation_signature == dvn.construct_signed_attestation_signature
+            && nodes.dv_pubkey == dvn.dv_pubkey       
+            && nodes.peers == dvn.all_nodes
+    }
+
+    predicate inv4(dvn: DVState)
+    {
         forall n: BLSPubkey | n in dvn.honest_nodes_states.Keys ::            
             && var nodes := dvn.honest_nodes_states[n];
             && forall duty: AttestationDuty | duty in nodes.all_rcvd_duties ::
@@ -1497,6 +1506,23 @@ module Att_Inv_With_Empty_Initial_Attestation_Slashing_DB
                     && dvn.sequence_attestation_duties_to_be_served[k].attestation_duty == duty
     }
 
+    predicate inv5(dvn: DVState)
+    {
+        forall hn: BLSPubkey | hn in dvn.honest_nodes_states.Keys ::            
+            && var dvc := dvn.honest_nodes_states[hn];
+            && ( dvc.current_attestation_duty.isPresent()
+                    ==> dvc.current_attestation_duty.safe_get()
+                            in dvc.all_rcvd_duties )
+    }
+
+    predicate inv6(dvn: DVState)
+    {
+        forall hn: BLSPubkey | hn in dvn.honest_nodes_states.Keys ::            
+            && var dvc := dvn.honest_nodes_states[hn];
+            && ( dvc.latest_attestation_duty.isPresent()
+                    ==> dvc.latest_attestation_duty.safe_get()
+                            in dvc.all_rcvd_duties )
+    }
 
 
     predicate invNetwork(
