src/dvspec/dafny/att_spec_proofs/dvn_init_inv.dfy
@@ -5,8 +5,10 @@ include "../specification/network.dfy"
 include "../specification/dvn.dfy"
 include "../att_spec_proofs/inv.dfy"
 include "../att_spec_proofs/assump.dfy"
+include "../att_spec_proofs/fnc_inv.dfy"
+include "../att_spec_proofs/helper_sets_lemmas.dfy"
 
-module DVN_Init_Ind_Inv
+module DVN_Init_Inv
 {
     import opened Types 
     import opened CommonFunctions
@@ -18,18 +20,6 @@ module DVN_Init_Ind_Inv
     import opened Att_Assumptions
 
     
-    lemma dvn_init_inv5(dvn: DVState)
-    requires && var initial_attestation_slashing_db: set<SlashingDBAttestation> := {}; 
-             && DV.Init(dvn, initial_attestation_slashing_db)    
-    ensures inv5(dvn)
-    {}
-
-    lemma dvn_init_inv10(dvn: DVState)
-    requires && var initial_attestation_slashing_db: set<SlashingDBAttestation> := {}; 
-             && DV.Init(dvn, initial_attestation_slashing_db)    
-    ensures inv5(dvn)
-    {}
-
     lemma dvn_init_inv1(dvn: DVState)       
     requires DV.Init(dvn, {})    
     ensures inv1(dvn)
@@ -62,5 +52,9 @@ module DVN_Init_Ind_Inv
     ensures inv3(dvn)
     {}    
 
+    lemma dvn_init_inv4(dvn: DVState)
+    requires DV.Init(dvn, {})    
+    ensures inv4(dvn)
+    {}
 
 }
