src/dvspec/dafny/att_spec_proofs/dvn_next_inv.dfy
@@ -5,11 +5,10 @@ include "../specification/network.dfy"
 include "../specification/dvn.dfy"
 include "../att_spec_proofs/inv.dfy"
 include "../att_spec_proofs/assump.dfy"
-include "../att_spec_proofs/dvc_ind_inv.dfy"
-include "../att_spec_proofs/fnc_ind_inv.dfy"
+include "../att_spec_proofs/fnc_inv.dfy"
 include "../att_spec_proofs/helper_sets_lemmas.dfy"
 
-module DVN_Next_Ind_Inv
+module DVN_Next_Inv
 {
     import opened Types 
     import opened CommonFunctions
@@ -19,72 +18,8 @@ module DVN_Next_Ind_Inv
     import opened DV
     import opened Att_Inv_With_Empty_Initial_Attestation_Slashing_DB
     import opened Att_Assumptions
-    import opened DVN_Ind_Inv
-    import opened Fnc_Ind_Inv
+    import opened Fnc_Inv
     import opened Helper_Sets_Lemmas
-
-    lemma {:axiom} dvn_next_event_inv5_axiom(dvn: DVState, e: DV.Event, dvn': DVState)       
-    requires DV.NextEvent(dvn, e, dvn')        
-    requires inv5(dvn)
-    ensures inv5(dvn')
-
-    lemma dvn_next_event_inv5(dvn: DVState, e: DV.Event, dvn': DVState)       
-    requires DV.NextEvent(dvn, e, dvn')        
-    requires inv5(dvn)
-    // ensures inv5(dvn')
-    {
-        if e.HonestNodeTakingStep?
-        {
-            var hn: BLSPubkey, hnEvent: Types.Event, hnOutputs: Outputs :| 
-                        NextHonestNode(dvn, hn, hnEvent, hnOutputs, dvn');
-            
-            var s_w_honest_node_states_updated :|
-                && ( if hnEvent.ImportedNewBlock? then 
-                                     
-                        s_w_honest_node_states_updated == 
-                            dvn.(
-                                honest_nodes_states := dvn.honest_nodes_states[hn := add_block_to_bn(dvn.honest_nodes_states[hn], hnEvent.block)]
-                            )
-                     
-                     else 
-                     
-                        s_w_honest_node_states_updated == dvn
-                     
-                   )
-                && NextHonestAfterAddingBlockToBn(s_w_honest_node_states_updated, hn, hnEvent, hnOutputs, dvn' )
-                ;
-
-            if hnEvent.ImportedNewBlock? 
-            {
-                assert s_w_honest_node_states_updated == 
-                            dvn.(
-                                honest_nodes_states := dvn.honest_nodes_states[hn := add_block_to_bn(dvn.honest_nodes_states[hn], hnEvent.block)]
-                            );
-                assert inv5(s_w_honest_node_states_updated);
-            }                 
-            else
-            {
-                assert s_w_honest_node_states_updated == dvn;
-                assert inv5(s_w_honest_node_states_updated);
-            }                    
-                        
-            assert inv5(s_w_honest_node_states_updated);     
-           
-            var hn_state := s_w_honest_node_states_updated.honest_nodes_states[hn];
-            var hn_state' := dvn'.honest_nodes_states[hn];
-            assert DVCNode_Spec.Next(hn_state, hnEvent, hn_state', hnOutputs);
-            assert inv5_body(hn_state);
-            dvc_next_inv5(hn_state, hn_state');
-            assert inv5_body(hn_state');
-           
-            // dvn_next_event_inv5_axiom(dvn, e, dvn');
-            // assert inv5(dvn');     
-        }
-        else
-        {
-            // dvn_next_event_inv5_axiom(dvn, e, dvn');
-        }        
-    }
 
     lemma lemma_dvn_next_inv1(dvn: DVState, dvn': DVState)       
     requires exists e: DV.Event :: DV.NextEvent(dvn, e, dvn')
@@ -98,22 +33,16 @@ module DVN_Next_Ind_Inv
     ensures inv2(dvn')
     { }
 
-    lemma {:axiom} assump_lemma_dvn_next_inv3(
-        s': DVState
-    )
-    ensures inv3(s')
-
     lemma lemma_dvn_next_inv3(
         dvn: DVState,
         event: DV.Event,
         dvn': DVState
     )
     requires inv1(dvn)
-    requires unchanged_fixed_paras(dvn, dvn')
     requires NextEvent(dvn, event, dvn')
     requires inv3(dvn)
     ensures inv3(dvn')
-    {
+    {        
         match event 
         {
             case HonestNodeTakingStep(node, nodeEvent, nodeOutputs) =>
